theories/PropBool.v
@@ -1,0 +1,97 @@
+Class PropBool1
+      {A: Type}
+      (pred: A -> Prop)
+      (pred_bool: A -> bool) :=
+  { pred_bool_pred_1 (a: A): pred_bool a = true <-> pred a
+  }.
+
+Lemma pred_bool_false_1
+      {A: Type}
+      (pred: A -> Prop)
+      (pred_bool: A -> bool)
+     `{PropBool1 A pred pred_bool}
+      (a: A)
+  : pred_bool a = false <-> ~pred a.
+Proof.
+  split.
+  + intros Hpred_bool Hpred.
+    apply (pred_bool_pred_1 a) in Hpred.
+    rewrite Hpred in Hpred_bool.
+    discriminate.
+  + intros Hnpred.
+    case_eq (pred_bool a); intro Heq.
+    ++ apply (pred_bool_pred_1 a) in Heq.
+       apply Hnpred in Heq.
+       destruct Heq.
+    ++ reflexivity.
+Qed.
+
+Class PropBool2
+      {A: Type}
+      {B: Type}
+      (pred: A -> B -> Prop)
+      (pred_bool: A -> B -> bool) :=
+  { pred_bool_pred_2 (a: A)
+                     (b: B)
+    : pred_bool a b = true <-> pred a b
+  }.
+
+Lemma pred_bool_false_2
+      {A: Type}
+      {B: Type}
+      (pred: A -> B -> Prop)
+      (pred_bool: A -> B -> bool)
+     `{PropBool2 A B pred pred_bool}
+      (a: A)
+      (b: B)
+  : pred_bool a b = false <-> ~pred a b.
+Proof.
+  split.
+  + intros Hpred_bool Hpred.
+    apply (pred_bool_pred_2 a b) in Hpred.
+    rewrite Hpred in Hpred_bool.
+    discriminate.
+  + intros Hnpred.
+    case_eq (pred_bool a b); intro Heq.
+    ++ apply (pred_bool_pred_2 a b) in Heq.
+       apply Hnpred in Heq.
+       destruct Heq.
+    ++ reflexivity.
+Qed.
+
+Class PropBool3
+      {A: Type}
+      {B: Type}
+      {C: Type}
+      (pred: A -> B -> C -> Prop)
+      (pred_bool: A -> B -> C -> bool) :=
+  { pred_bool_pred_3 (a: A)
+                     (b: B)
+                     (c: C)
+    : pred_bool a b c = true <-> pred a b c
+  }.
+
+Lemma pred_bool_false_3
+      {A: Type}
+      {B: Type}
+      {C: Type}
+      (pred: A -> B -> C -> Prop)
+      (pred_bool: A -> B -> C -> bool)
+     `{PropBool3 A B C pred pred_bool}
+      (a: A)
+      (b: B)
+      (c: C)
+  : pred_bool a b c = false <-> ~pred a b c.
+Proof.
+  split.
+  + intros Hpred_bool Hpred.
+    apply (pred_bool_pred_3 a b c) in Hpred.
+    rewrite Hpred in Hpred_bool.
+    discriminate.
+  + intros Hnpred.
+    case_eq (pred_bool a b c); intro Heq.
+    ++ apply (pred_bool_pred_3 a b c) in Heq.
+       apply Hnpred in Heq.
+       destruct Heq.
+    ++ reflexivity.
+Qed.
